% Problem 3/6 solution
\noindent
\underline{Solution:}\\

\noindent
Use the variational principle and employ spherical coordinates in integrations:\\

$E = \frac{\int\psi^*_{trial}H\psi_{trial}d\tau}{\int\psi^*_{trial}\psi_{trial}d\tau}$

\noindent
a)
$$\int\psi^*_{trial}\psi_{trial}d\tau = \int_0^\infty e^{-2kr}
\underbrace{4\pi r^2dr}_{d\tau} = 4\pi\int_0^\infty r^2e^{-2kr}dr
= \frac{\pi}{k^3}$$

$$\int\psi_{trial}^*H\psi_{trial}d\tau = \int\left( e^{-kr}\right)
\left( -\frac{\hbar^2}{2m_e}\Delta - \frac{e^2}{4\pi\epsilon_0r}\right)
\left( e^{-kr}\right)d\tau$$

$$= \int_0^\infty\left( e^{-kr}\right)
\left( -\frac{\hbar^2}{2m_e}\left[\frac{\partial^2}{\partial r^2} + \frac{2}{r}\frac{\partial}
{\partial r}\right] - \frac{e^2}{4\pi\epsilon_0r}\right)\left( e^{-kr}\right)
\left( 4\pi r^2dr\right)$$

$$= -\frac{4\pi\hbar^2}{2m_e}\int_0^\infty \left( e^{-kr}\right)
\left( k^2e^{-kr} - \frac{2k}{r}e^{-kr}\right)r^2dr 
- \frac{e^2}{\epsilon_0}\int_0^\infty\frac{e^{-2kr}}{r}r^2dr$$

$$= -\frac{4\pi\hbar^2}{2m_e}\int_0^\infty e^{-2kr}(r^2k^2 - 2kr)dr
- \frac{e^2}{\epsilon_0}\int_0^\infty re^{-2kr}dr$$

$$= -\frac{2\pi\hbar^2k^2}{m_e}\underbrace{\int_0^\infty r^2 e^{-2kr}dr}_{= \frac{2}{(2k)^3}}
+ \frac{4\pi\hbar^2k}{m_e}\underbrace{\int_0^\infty re^{-2kr}dr}_{= 
\frac{1}{(2k)^2}} - \frac{e^2}{\epsilon_0}\underbrace{\int_0^\infty
re^{-2kr}dr}_{= \frac{1}{(2k)^2}}$$

$$= -\frac{\pi\hbar^2}{2m_ek} + \frac{\pi\hbar^2}{m_ek}
- \frac{e^2}{4k^2\epsilon_0}$$

\noindent
These results give:\\

$$\frac{\int\psi^*H\psi d\tau}{\int\psi^*\psi d\tau} =
\left( -\frac{\pi\hbar^2}{2m_ek} + \frac{\pi\hbar^2}{m_ek}
- \frac{e^2}{4k^2\epsilon_0}\right) / \left( \pi / k^3\right)$$

$$ = -\frac{\hbar^2k^2}{2m_e} + \frac{\hbar^2k^2}{m_e} - \frac{e^2k}
{4\pi\epsilon_0} = \frac{\hbar^2k^2}{2m_e} - \frac{e^2k}{4\pi\epsilon_0}$$\\

\noindent
This expression must be minimized with respect to variational parameter
$k$:\\

$$\frac{dE}{dk} = d\left( \frac{\hbar^2k^2}{2m_e} - \frac{e^2k}
{4\pi\epsilon_0}\right) / dk = \frac{\hbar^2k}{m_e} - \frac{e^2}
{4\pi\epsilon_0} = 0$$

$$\Rightarrow k = \frac{m_ee^2}{4\pi\epsilon_0\hbar^2} \Rightarrow
E = -\frac{1}{2}\frac{m_ee^4}{(4\epsilon_0)^2\hbar^2} = -hcR$$

\noindent
where $R$ is the Rydberg constant.\\

\noindent
b) The logic is exactly the same as in part a).\\

$$\int\psi^*_{trial}\psi_{trial}d\tau = \int_0^\infty e^{-2kr^2}
\underbrace{4\pi r^2dr}_{d\tau} = \frac{4\pi\Gamma[3/2]}{2(2k)^{3/2}}
= \frac{\pi^{3/2}}{(2k)^{3/2}}$$

\noindent
The Laplacian of this function is given by:

$$\Delta\psi_{trial} = \frac{\partial}{\partial r}\left( -2kre^{-kr^2}
\right) + \frac{2}{r}\left( -2kr\right)e^{-kr^2} = \left( 4k^2r^2
- 6k\right) e^{-kr^2}$$

\noindent
Thus the energy expectation value is (without normalization):\\

$$\int_o^\infty\left( -\frac{2\hbar^2k^2r^2}{m_e} + \frac{3k\hbar^2}
{m_e} - \frac{e^2}{4\pi\epsilon_0}\frac{1}{r}\right)e^{-2kr^2}\times
4\pi r^2dr$$

$$= 4\pi\int_0^\infty\left( -\frac{2\hbar^2k^2r^4}{m_e} 
+ \frac{3k\hbar^2r^2}{m_e} - \frac{e^2r}{4\pi\epsilon_0}\right) e^{-2kr^2}dr$$

$$= -\frac{8\pi\hbar^2k^2}{m_e}\underbrace{\int_0^\infty r^4 
e^{-2kr^2}dr}_{\frac{\Gamma[5/2]}{2(2k)^{5/2}} = \frac{3\sqrt{\pi}}{8(2k)^{5/2}}}
+ \underbrace{\frac{12\pi k\hbar^2}{m_e}\int_o^\infty 
r^2e^{-2kr^2}dr}_{\frac{\Gamma[3/2]}{2(2k)^{3/2}} = \frac{\sqrt{\pi}}{4(2k)^{3/2}}}
- \frac{e^2}{\epsilon_0}\underbrace{\int_0^\infty 
re^{-2kr^2}dr}_{\frac{\Gamma[1]}{2(2k)} = 1/(4k)}
$$

$$= - \frac{3\pi^{3/2}\hbar^2}{4m_e\sqrt{2k}} + \frac{3\pi^{3/2}\hbar^2}
{2m_e\sqrt{2k}} - \frac{e^2}{4\epsilon_0k}$$

$$\Rightarrow \frac{\int\psi^*_{trial}\psi_{trial}d\tau}
{\int\psi^*_{trial}\psi_{trial}d\tau} 
= \frac{-\frac{3\pi^{3/2}\hbar^2}{4m_e\sqrt{2k}} + \frac{3\pi^{3/2}\hbar^2}
{2m_e\sqrt{2k}} - \frac{e^2}{4\epsilon_0k}}{\frac{\pi^{3/2}}{(2k)^{3/2}}}
= -\frac{3\hbar^2k}{2m_e} + \frac{6\hbar^2k}{2m_e} - \frac{e^2\sqrt{2k}}
{2\pi^{3/2}\epsilon_0}
$$

$$= \frac{3\hbar^2k}{2m_e} - \frac{e^2\sqrt{k}}{\sqrt{2}\pi^{3/2}\epsilon_0}$$

\noindent
To find the minimum value for energy (with respect to $k$), we calculate
the first derivative and set it to zero:\\

$$E = \frac{3\hbar^2k}{2m_e} - \frac{e^2\sqrt{k}}{\sqrt{2}\pi^{3/2}\epsilon_0}$$

$$\Rightarrow \frac{\partial E}{\partial k} = \frac{3\hbar^2}{2m_e}
- \frac{e^2}{2\sqrt{2}\pi^{3/2}\epsilon_0\sqrt{k}} = 0$$

$$\Rightarrow k=\left(\frac{m_ee^2}{3\sqrt{2}\pi^{3/2}\epsilon_0\hbar^2}
\right)^2 = \frac{m_e^2e^4}{18\pi^3\epsilon_0^2\hbar^4}$$

\noindent
The total energy at this point is:

$$E = \frac{3\hbar^2}{2m_e}\times\frac{m_e^2e^4}{18\pi^3\epsilon_0^2
\hbar^4} - \frac{e^2}{\sqrt{2}\pi^{3/2}\epsilon_0}\times
\frac{m_ee^2}{3\sqrt{2}\pi^{3/2}\epsilon_0\hbar^2}
= \frac{m_ee^4}{12\pi^3\epsilon_0^2\hbar^2} - \frac{2m_ee^4}
{12\pi^3\epsilon^2_0\hbar^2}$$

$$ = -\frac{m_ee^4}{12\pi^3\epsilon_0^2\hbar^2} = -\frac{8}{3\pi}hcR \approx -0.85hcR$$\\

\noindent
c) The function in a) gives lower energy and therefore that trial function
is better.\\

\hrule\vspace{0.5cm}
