% Problem 9/1 solution
\noindent
\underline{Solution:}\\

\begin{itemize}

\item[a)] $$\left(\frac{\partial P}{\partial V}\right)_T = -\frac{nRT}{\left(V - nb\right)^2}\textnormal{ and }\left(\frac{\partial P}{\partial T}\right)_V = \frac{nR}{V - nb}$$

\item[b)] $$\left(\frac{\partial^2P}{\partial V\partial T}\right) = -\frac{nR}{\left(V - nb\right)^2}\textnormal{ and }\left(\frac{\partial^2P}{\partial T\partial V}\right) = -\frac{nR}{\left(V - nb\right)^2}$$

\end{itemize}
\hrule\vspace{0.5cm}
