% Problem 4/6 solution
\noindent
\underline{Solution:}

Because $G = G(g) + G(l)$ and $dG = 0$, we have: $dG = dG(g) + dG(l) = 0$. Furthermore, for both liquid and gas, we have:

$$dG(l) = \mu_A(l)dn_A(l) + \mu_B(l)dn_B(l)$$
$$dG(g) = \mu_A(g)dn_A(g) + \mu_B(g)dn_B(g)$$

Because $dn_A(l) = -dn_A(g)$ and $dn_B(l) = -dn_B(g)$, we get:
$$dG = dG(l) + dG(g) = \left(\mu_A(g) - \mu_A(l)\right)dn_A(g) + \left(\mu_B(g) - \mu_B(l)\right)dn_B(g) = 0$$

Both $dn_A(g)$ and $dn_B(g)$ can be varied independently, which means that the coefficients in front of them must both be zero:
$$\mu_A(g) - \mu_A(l) = 0\textnormal{ and }\mu_B(g) - \mu_B(l) = 0\Rightarrow \mu_A(g) = \mu_A(l)\textnormal{ and }\mu_B(g) = \mu_B(l)$$

\hrule\vspace{0.5cm}
